src/program_proof/simplepb/primary_protocol.v
@@ -58,16 +58,16 @@ Definition own_escrow_toks γsrv epoch : iProp Σ :=
   [∗ set] epoch' ∈ (fin_to_set u64), ⌜int.nat epoch' ≤ int.nat epoch⌝ ∨ own_tok γsrv epoch'
 .
 
-Definition own_primary_ghost γsys γsrv (canBecomePrimary:bool) epoch : iProp Σ :=
+Definition own_primary_escrow_ghost γsys γsrv (canBecomePrimary:bool) epoch : iProp Σ :=
   "Htoks" ∷ own_escrow_toks γsrv epoch ∗
   "Htok" ∷ (if canBecomePrimary then own_tok γsrv epoch else True)
 .
 
 Lemma ghost_primary_accept_new_epoch γsys γsrv epoch canBecomePrimary epoch' :
   int.nat epoch < int.nat epoch' →
-  own_primary_ghost γsys γsrv canBecomePrimary epoch
+  own_primary_escrow_ghost γsys γsrv canBecomePrimary epoch
   ==∗
-  own_primary_ghost γsys γsrv true epoch'.
+  own_primary_escrow_ghost γsys γsrv true epoch'.
 Proof.
   (*
   intros Hineq.
@@ -126,9 +126,9 @@ Lemma ghost_become_primary γsys γsrv epoch σprop σ R :
   £ 1 -∗
   become_primary_escrow γsys γsrv epoch σprop R -∗
   is_proposal_facts_prim γsys epoch σ -∗
-  own_primary_ghost γsys γsrv true epoch ={↑pbN}=∗
+  own_primary_escrow_ghost γsys γsrv true epoch ={↑pbN}=∗
   ⌜σprop ⪯ σ⌝ ∗
-  own_primary_ghost γsys γsrv false epoch ∗
+  own_primary_escrow_ghost γsys γsrv false epoch ∗
   R
 .
 Proof.
